proofs/arch/sem_params_of_arch_extra.v
@@ -11,13 +11,14 @@ Section SEM_PARAMS.
     {reg regx xreg rflag cond asm_op extra_op : Type}
     {asm_e : asm_extra reg regx xreg rflag cond asm_op extra_op}
     {syscall_state : Type}
-  .
+    {scs : syscall_sem syscall_state}.
 
   (* In the proofs where we have an architecture instance, we always have a
      syscall semantics. Forcing the dependency on [scs] makes inference more
      convenient. *)
   #[export]
-  Instance ep_of_asm_e : EstateParams syscall_state :=
+  Instance ep_of_asm_e {_ : syscall_sem syscall_state} :
+    EstateParams syscall_state :=
     {
       _pd := arch_pd;
       _msf_size := arch_msfsz;
@@ -33,6 +34,7 @@ Section SEM_PARAMS.
   Instance sip_of_asm_e : SemInstrParams extended_op syscall_state :=
     {
       _asmop := asm_opI;
+      _sc_sem := scs;
     }.
 
 End SEM_PARAMS.
